Eval.v
@@ -1,0 +1,74 @@
+Require Import STLC.
+Require Import TypeChecker.
+Require Import EqNat.
+
+Fixpoint substitute (var: nat) (e body: STLCExpr) :=
+  match body with
+  | Lambda t lVar lBody =>
+      if beq_nat lVar var then
+        Lambda t lVar lBody
+      else
+        Lambda t lVar (substitute var e lBody)
+  | If c tBranch eBranch =>
+      If (substitute var e c) (substitute var e tBranch) (substitute var e eBranch)
+  | Var otherV =>
+      if beq_nat otherV var then
+        e
+      else
+        Var otherV
+  | App e1 e2 => App (substitute var e e1) (substitute var e e2)
+  | v => v
+  end
+.
+
+Fixpoint evalStep (e: STLCExpr) : (option STLCExpr) :=
+  match e with
+  | If cond tBranch eBranch =>
+    match cond with
+    | True => Some tBranch
+    | False => Some eBranch
+    | c => match evalStep c with
+            | Some c' => Some (If c' tBranch eBranch)
+            | None => None
+          end
+    end
+  | App e1 e2 =>
+    match e1 with
+      | Lambda _ var body => Some (substitute var e2 body)
+      | _ => None
+    end
+  | _ => None
+  end
+.
+
+(* TAPL page 105-106 *)
+Theorem wellTypedProgress: forall (e: STLCExpr) (T: STLCType),
+    type_of e (M.empty STLCType) = Some T
+    -> isValue e = true \/ exists e', evalStep e = Some e'.
+Proof.
+  intros e.
+  induction e.
+  - left. reflexivity.
+  - left. reflexivity.
+  - left. reflexivity.
+  - right. symmetry in H. apply inversion_6 in H.
+    destruct H. destruct H0. rewrite <- H0 in IHe3.
+    clear H0. assert (H0 := H1). assert (H' := H).
+    * apply IHe1 in H. apply IHe3 in H0. apply IHe2 in H1.
+      destruct H.
+      + apply cannonical_form1 in H'. destruct H'.
+          simpl. rewrite H2. exists e2. reflexivity.
+          simpl. rewrite H2. exists e3. reflexivity.
+          assumption.
+      + simpl. destruct e1; eauto;
+        destruct H; rewrite H; exists (If x e2 e3); reflexivity.
+  - right. inversion H.
+  - right. symmetry in H. apply inversion_3 in H. inversion H. inversion H0.
+    destruct H1. destruct H2. assert (H2' := H2). apply IHe1 in H2. apply IHe2 in H3.
+    destruct H2.
+    * rewrite H1 in H2'. apply canonical_form2 in H2'. destruct H2'. destruct H4.
+      simpl. rewrite H4. exists (substitute x1 e2 x2).
+      + reflexivity.
+      + assumption.
+    * rewrite H1 in H2'. destruct H2.
+Qed.
